Added unit_unique axiom

LogicalRefinement/Typed/Basic.lean
@@ -377,6 +377,9 @@ inductive HasType: Context -> Term -> Annot -> Prop
     HasType Γ.upgrade a (term A) -> HasType Γ.upgrade b (term B) ->
     HasType Γ p (proof (eq (coprod A B) (inj 0 a) (inj 1 b))) ->
     HasType Γ (discr a b p) (proof bot)
+  | unit_unique {Γ: Context} {a: Term}:
+    HasType Γ.upgrade a (term unit) ->
+    HasType Γ (unit_unique a) (proof (eq unit a nil))
   | cong {Γ: Context} {A P p e x y: Term}:
     HasType ((Hyp.mk A (HypKind.val type))::Γ) P prop -> 
     HasType Γ A type ->
