LogicalRefinement/Untyped/Basic.lean
@@ -82,6 +82,7 @@ inductive TermKind: List Nat -> Type
   | eq: TermKind [0, 0, 0]
   | refl: TermKind [0]
   | discr: TermKind [0, 0, 0]
+  | unit_unique: TermKind [0]
   | cong: TermKind [0, 0, 1]
   | trans: TermKind [0, 0, 1]
   | beta: TermKind [0, 1]
@@ -175,6 +176,7 @@ abbrev Term.let_wit := let_bin TermKind.let_wit
 -- Theory of equality
 abbrev Term.refl := unary TermKind.refl
 abbrev Term.discr := tri TermKind.discr
+abbrev Term.unit_unique := unary TermKind.unit_unique
 abbrev Term.cong := ir TermKind.cong
 abbrev Term.trans := ir TermKind.trans
 abbrev Term.beta := abs TermKind.beta
